src/Distributions/BernoulliExpNeg/Correctness.dfy
@@ -13,8 +13,4 @@ module BernoulliExpNeg.Correctness {
   lemma {:axiom} Correctness(gamma: Rationals.Rational)
     requires 0 <= gamma.numer
     ensures Rand.prob(iset s | Model.Sample(gamma)(s).Equals(true)) == Exponential.Exp(-Rationals.ToReal(gamma))
-
-  lemma {:axiom} SampleIsIndep(gamma: Rationals.Rational)
-    requires 0 <= gamma.numer
-    ensures Independence.IsIndep(Model.Sample(gamma))
 }
